start entropy theorem, try to figure out abstraction function version / how to deal with streams

specs/DRBG_generate_function.v
@@ -7,40 +7,145 @@ Require Import DRBG_generate_algorithm_result.
 Require Import DRBG_reseed_function.
 Require Import entropy.
 
-Fixpoint DRBG_generate_function_helper (generate_algorithm: DRBG_working_state -> Z -> list Z -> DRBG_generate_algorithm_result) (reseed_function: ENTROPY.stream -> DRBG_state_handle -> bool -> list Z -> ENTROPY.result DRBG_state_handle) (entropy_stream: ENTROPY.stream) (state_handle: DRBG_state_handle) (requested_number_of_bytes: Z) (prediction_resistance_request: bool) (additional_input: list Z) (should_reseed: bool) (count: nat): ENTROPY.result (list Z * DRBG_working_state) :=
+(* 12/15/15
+
+new fn: how many bits of entropy it consumed
+prefix of that length that relates the two infinite streams
+abstraction function
+will need to have all of these (orange) parameters
+
+stream = exists finite prefix of size n ++ stream'
+
+see naphat's entropy.v
+
+but how do i use the abstraction function??
+what's the new theorem statement?
+
+(also, how do i deal with the failures in the stream?)
+
+? i don't remember what else
+
+do i need some relation on the input stream? or just equality?
+
+DRBG_generate_function_helper' ga rf stream state n prr ai reseed ct :=
+  min_bits
+
+f $ DRBG_gen inputs = DRBG_gen' inputs
+
+note: stream in (entropy_stream), stream out (ENTROPY.result)
+
+wouldn't it be an abstraction theorem instead?
+would definitely need to reason about low-level parts of naphat's spec
+
+would i need an abstraction function/theorem for reseed as well? since it actually calls GE
+
+need to do the abstraction function on the stream of all successes
+
+gen_func (filter entropy_stream) .. other inputs .. = entropy_stream' .. other outputs ..
+is the filtering ok?
+
+gen_func (filter entropy_stream) .. other inputs ..
+is equivalent to
+calling gen_func repeatedly until n successes? 
+
+and then gen_func (filter entropy_stream) = 
+
+should i say "after n generate calls, the stream returned is equal to the original stream with the first (e * 1 + (l/r)) bits removed"?
+
+prove that after 1 generate call
+(maybe i shouldn't be thinking in terms of # calls???)
+___???
+
+
+
+if the entropy fails, then the reseed fails, the gen func helper fails, and the gen func fails (up to the top level). so, i have to deal with calling generate until there is a success. that might not terminate? 
+
+Inductive result X: Type: Type :=
+| success: X -> stream -> @result X
+| error : error_code -> stream -> @result X.
+
+ *)
+Fixpoint DRBG_generate_function_helper
+         (generate_algorithm: DRBG_working_state -> Z -> list Z
+                              -> DRBG_generate_algorithm_result)
+         (reseed_function: ENTROPY.stream -> DRBG_state_handle
+                           -> bool -> list Z -> ENTROPY.result DRBG_state_handle)
+         (entropy_stream: ENTROPY.stream)
+         (state_handle: DRBG_state_handle)
+         (requested_number_of_bytes: Z)
+         (prediction_resistance_request: bool)
+         (additional_input: list Z)
+         (should_reseed: bool)
+         (count: nat): ENTROPY.result (list Z * DRBG_working_state) :=
+  (* reseed happens here on second call to helper *)
   let result := if should_reseed then
-                        match reseed_function entropy_stream state_handle prediction_resistance_request additional_input with
-                          | ENTROPY.success x entropy_stream => ENTROPY.success (x, []) entropy_stream
-                          | ENTROPY.error e entropy_stream => ENTROPY.error e entropy_stream
-                        end
-                      else ENTROPY.success (state_handle, additional_input) entropy_stream in
+                  (* passes the entropy stream to the reseed function *)
+                  match reseed_function entropy_stream state_handle
+                                        prediction_resistance_request
+                                        additional_input with
+                  | ENTROPY.success x entropy_stream =>
+                    ENTROPY.success (x, []) entropy_stream
+                  | ENTROPY.error e entropy_stream =>
+                    ENTROPY.error e entropy_stream
+                  end
+                else ENTROPY.success (state_handle, additional_input) entropy_stream in
   match result with
     | ENTROPY.error e s => ENTROPY.error e s
     | ENTROPY.success (state_handle, additional_input) entropy_stream =>
       let '(working_state, security_strength, prediction_resistance_flag) := state_handle in
+      (* generate_algorithm actually called here *)
       match generate_algorithm working_state requested_number_of_bytes additional_input with
         | generate_algorithm_reseed_required =>
           match count with
             | O => ENTROPY.error ENTROPY.generic_error entropy_stream (* impossible *)
-            | S count' => DRBG_generate_function_helper generate_algorithm reseed_function entropy_stream state_handle requested_number_of_bytes prediction_resistance_request additional_input true count'
+            | S count' =>
+              (* reseed happens here -- calls helper again *)
+              DRBG_generate_function_helper
+                generate_algorithm reseed_function entropy_stream state_handle
+                requested_number_of_bytes prediction_resistance_request additional_input
+                true count'
           end
         | generate_algorithm_success x y => ENTROPY.success (x, y) entropy_stream
       end
     end.
 
-Definition DRBG_generate_function (generate_algorithm: Z -> DRBG_working_state -> Z -> list Z -> DRBG_generate_algorithm_result) (reseed_function: ENTROPY.stream -> DRBG_state_handle -> bool -> list Z -> ENTROPY.result DRBG_state_handle) (reseed_interval: Z) (max_number_of_bytes_per_request: Z) (max_additional_input_length: Z) (entropy_stream: ENTROPY.stream) (state_handle: DRBG_state_handle) (requested_number_of_bytes requested_security_strength: Z) (prediction_resistance_request: bool) (additional_input: list Z): ENTROPY.result (list Z * DRBG_state_handle) :=
+Definition DRBG_generate_function
+           (generate_algorithm: Z -> DRBG_working_state -> Z -> list Z
+                                -> DRBG_generate_algorithm_result)
+           (reseed_function: ENTROPY.stream -> DRBG_state_handle -> bool
+                             -> list Z -> ENTROPY.result DRBG_state_handle)
+           (reseed_interval: Z)
+           (max_number_of_bytes_per_request: Z)
+           (max_additional_input_length: Z)
+           (entropy_stream: ENTROPY.stream)
+           (state_handle: DRBG_state_handle)
+           (requested_number_of_bytes requested_security_strength: Z)
+           (prediction_resistance_request: bool)
+           (additional_input: list Z):
+  ENTROPY.result (list Z * DRBG_state_handle) :=
   let '(working_state, security_strength, prediction_resistance_flag) := state_handle in
-  if Z.gtb requested_number_of_bytes max_number_of_bytes_per_request then ENTROPY.error ENTROPY.generic_error entropy_stream
+  if Z.gtb requested_number_of_bytes max_number_of_bytes_per_request 
+  then ENTROPY.error ENTROPY.generic_error entropy_stream
   else
-    if Z.gtb requested_security_strength security_strength then ENTROPY.error ENTROPY.generic_error entropy_stream
+    if Z.gtb requested_security_strength security_strength 
+    then ENTROPY.error ENTROPY.generic_error entropy_stream
     else
-      if Z.gtb (Zlength additional_input) max_additional_input_length then ENTROPY.error ENTROPY.generic_error entropy_stream
+      if Z.gtb (Zlength additional_input) max_additional_input_length 
+      then ENTROPY.error ENTROPY.generic_error entropy_stream
       else
-        if prediction_resistance_request && (negb prediction_resistance_flag) then ENTROPY.error ENTROPY.generic_error entropy_stream
+        if prediction_resistance_request && (negb prediction_resistance_flag) 
+        then ENTROPY.error ENTROPY.generic_error entropy_stream
         else
-          match DRBG_generate_function_helper (generate_algorithm reseed_interval) reseed_function entropy_stream state_handle requested_number_of_bytes prediction_resistance_request additional_input prediction_resistance_request 1%nat with
+          (* helper used here *)
+          match DRBG_generate_function_helper
+                  (* generate_algorithm here *)
+                  (generate_algorithm reseed_interval) reseed_function entropy_stream
+                  state_handle requested_number_of_bytes prediction_resistance_request
+                  additional_input prediction_resistance_request 1%nat with
             | ENTROPY.error e s => ENTROPY.error e s
-                                                 | ENTROPY.success (output, new_working_state) entropy_stream =>
-                                                   ENTROPY.success (output, (new_working_state, security_strength, prediction_resistance_flag)) entropy_stream
+            | ENTROPY.success (output, new_working_state) entropy_stream =>
+              ENTROPY.success (output, (new_working_state, security_strength,
+                                        prediction_resistance_flag))
+                              entropy_stream
           end.
 
