specs/DRBG_instantiate_function.v
@@ -5,19 +5,40 @@ Require Import DRBG_working_state.
 Require Import DRBG_state_handle.
 Require Import entropy.
 
-Definition DRBG_instantiate_function (instantiate_algorithm: list Z -> list Z -> list Z -> Z -> DRBG_working_state) (min_entropy_length max_entropy_length: Z) (get_nonce: unit -> list Z) (highest_supported_security_strength: Z) (max_personalization_string_length: Z) (prediction_resistance_supported: bool) (entropy_stream: ENTROPY.stream) (requested_instantiation_security_strength: Z) (prediction_resistance_flag: bool) (personalization_string: list Z): ENTROPY.result DRBG_state_handle :=
-  if Z.gtb requested_instantiation_security_strength highest_supported_security_strength then ENTROPY.error ENTROPY.generic_error entropy_stream
+(* API spec? *)
+Definition DRBG_instantiate_function 
+           (instantiate_algorithm: list Z -> list Z -> list Z -> Z -> DRBG_working_state) 
+           (min_entropy_length max_entropy_length: Z) 
+           (get_nonce: unit -> list Z) 
+           (highest_supported_security_strength: Z) 
+           (max_personalization_string_length: Z) 
+           (prediction_resistance_supported: bool) 
+           (entropy_stream: ENTROPY.stream) 
+           (requested_instantiation_security_strength: Z) 
+           (prediction_resistance_flag: bool) 
+           (personalization_string: list Z): ENTROPY.result DRBG_state_handle :=
+  if Z.gtb requested_instantiation_security_strength highest_supported_security_strength
+  then ENTROPY.error ENTROPY.generic_error entropy_stream
   else match prediction_resistance_flag, prediction_resistance_supported with
          | true, false => ENTROPY.error ENTROPY.generic_error entropy_stream
-         | _,_ =>
-           if Z.gtb (Zlength personalization_string) max_personalization_string_length then ENTROPY.error ENTROPY.generic_error entropy_stream
+         | _ , _ =>
+           if Z.gtb (Zlength personalization_string) max_personalization_string_length
+           then ENTROPY.error ENTROPY.generic_error entropy_stream
            else
-             let security_strength := requested_instantiation_security_strength in (* TODO actually follow specs *)
-             match get_entropy security_strength min_entropy_length max_entropy_length prediction_resistance_flag entropy_stream with
+             let security_strength := requested_instantiation_security_strength in
+             (* TODO actually follow specs *)
+             (* here get_entropy returns min_entropy_length entropy *)
+             match get_entropy security_strength min_entropy_length
+                               max_entropy_length prediction_resistance_flag
+                               entropy_stream with
                | ENTROPY.error e s' => ENTROPY.error ENTROPY.catastrophic_error s'
                | ENTROPY.success entropy_input entropy_stream =>
                  let nonce := get_nonce tt in
-                 let initial_working_state := instantiate_algorithm entropy_input nonce personalization_string security_strength in
-                 ENTROPY.success (initial_working_state, security_strength, prediction_resistance_flag) entropy_stream
+                 let initial_working_state :=
+                     (* actual instantiate algorithm is called here *)
+                     instantiate_algorithm entropy_input nonce
+                                           personalization_string security_strength in
+                 ENTROPY.success (initial_working_state, security_strength,
+                                  prediction_resistance_flag) entropy_stream
              end
        end.
