specs/DRBG_reseed_function.v
@@ -4,15 +4,32 @@ Require Import DRBG_state_handle.
 Require Import DRBG_working_state.
 Require Import entropy.
 
-Definition DRBG_reseed_function (reseed_algorithm: DRBG_working_state -> list Z -> list Z -> DRBG_working_state) (min_entropy_length max_entropy_length: Z) (max_additional_input_length: Z) (entropy_stream: ENTROPY.stream) (state_handle: DRBG_state_handle) (prediction_resistance_request: bool) (additional_input: list Z): ENTROPY.result DRBG_state_handle :=
+Definition DRBG_reseed_function 
+           (reseed_algorithm: DRBG_working_state -> list Z -> list Z -> DRBG_working_state) 
+           (min_entropy_length max_entropy_length: Z) 
+           (max_additional_input_length: Z) 
+           (entropy_stream: ENTROPY.stream) 
+           (state_handle: DRBG_state_handle) 
+           (prediction_resistance_request: bool) 
+           (additional_input: list Z): ENTROPY.result DRBG_state_handle :=
+
   let '(working_state, security_strength, prediction_resistance_flag) := state_handle in
-  if prediction_resistance_request && (negb prediction_resistance_flag) then ENTROPY.error ENTROPY.generic_error entropy_stream
+
+  if prediction_resistance_request && (negb prediction_resistance_flag) 
+  then ENTROPY.error ENTROPY.generic_error entropy_stream
   else
-    if Z.gtb (Zlength additional_input) max_additional_input_length then ENTROPY.error ENTROPY.generic_error entropy_stream
+    if Z.gtb (Zlength additional_input) max_additional_input_length 
+    then ENTROPY.error ENTROPY.generic_error entropy_stream
     else
-      match get_entropy security_strength min_entropy_length max_entropy_length prediction_resistance_flag entropy_stream with
-        | ENTROPY.error _ s => ENTROPY.error ENTROPY.catastrophic_error s
-        | ENTROPY.success entropy_input entropy_stream =>
-          let new_working_state := reseed_algorithm working_state entropy_input additional_input in
-          ENTROPY.success (new_working_state, security_strength, prediction_resistance_flag) entropy_stream
+      (* get_entropy finally called here *)
+      match get_entropy security_strength min_entropy_length
+                        max_entropy_length prediction_resistance_flag entropy_stream with
+      | ENTROPY.error _ s =>
+        ENTROPY.error ENTROPY.catastrophic_error s
+      | ENTROPY.success entropy_input entropy_stream =>
+        (* reseed_algorithm called here -- i'm guessing entropy_input has length > min *)
+        let new_working_state := reseed_algorithm working_state
+                                                  entropy_input additional_input in
+        ENTROPY.success (new_working_state, security_strength,
+                         prediction_resistance_flag) entropy_stream
       end.
